prepare for implementation type and relation depending on each other

src/cddl/pulse/CDDL.Pulse.AST.Types.fst
@@ -46,94 +46,61 @@ let rel_elem_type_sem
   | TTAlwaysFalse -> rel_always_false _ _
 
 [@sem_attr]
-type target_impl_env (bound: name_env) =
-  (typ_name bound -> Tot Type0)
+noeq
+type target_impl_sem (sem_spec_type: Type0) = {
+  sem_impl_type: Type0;
+  sem_rel: rel sem_impl_type sem_spec_type;
+}
+
+[@sem_attr]
+type rel_env
+  (#bound: name_env)
+  (s_env: target_type_env bound)
+= (n: typ_name bound) -> target_impl_sem (s_env.te_type n)
 
 [@sem_attr]
 let rec impl_type_sem
   (#bound: name_env)
-  (cbor_t: Type0)
-  (env: target_impl_env bound)
-  (t: target_type)
-: Pure Type0
+  (#cbor_t: Type0)
+  (vmatch: perm -> cbor_t -> Cbor.cbor -> slprop)
+  (#s_env: target_type_env bound)
+  (env: rel_env s_env)
+  (t: target_type { target_type_bounded bound t })
+: Pure (target_impl_sem (target_type_sem s_env.te_type t))
     (requires target_type_bounded bound t)
     (ensures fun _ -> True)
     (decreases t)
 = match t with
   | TTDef s -> env s
-  | TTElem elt -> impl_elem_type_sem cbor_t elt
-  | TTOption t -> option (impl_type_sem cbor_t env t)
-  | TTPair t1 t2 -> (impl_type_sem cbor_t env t1 & impl_type_sem cbor_t env t2)
-  | TTUnion t1 t2 -> either (impl_type_sem cbor_t env t1) (impl_type_sem cbor_t env t2)
-  | TTArray t -> slice (impl_type_sem cbor_t env t) // TODO: allow iterable CBOR array objects
-  | TTTable t1 t2 -> slice (impl_type_sem cbor_t env t1 & impl_type_sem cbor_t env t2) // TODO: allow iterable CBOR map objects
-
-let target_impl_env_included
-  (#bound1: name_env)
-  (s_env1: target_impl_env bound1)
-  (#bound2: name_env)
-  (s_env2: target_impl_env bound2)
-: Tot prop
-= name_env_included bound1 bound2 /\
-  (forall (x: typ_name bound1) . s_env1 x == s_env2 x)
-
-let rec impl_type_sem_incr
-  (#bound1: name_env)
-  (cbor_t: Type0)
-  (env1: target_impl_env bound1)
-  (#bound2: name_env)
-  (env2: target_impl_env bound2)
-  (t: target_type)
-: Lemma
-  (requires (target_impl_env_included env1 env2 /\
-    target_type_bounded bound1 t
-  ))
-  (ensures (
-    impl_type_sem cbor_t env1 t == impl_type_sem cbor_t env2 t
-  ))
-  [SMTPatOr [
-    [SMTPat (target_impl_env_included env1 env2); SMTPat (impl_type_sem cbor_t env1 t);];
-    [SMTPat (target_impl_env_included env1 env2); SMTPat (impl_type_sem cbor_t env2 t);];
-  ]]
-= match t with
-  | TTOption t1
-  | TTArray t1
-    -> impl_type_sem_incr cbor_t env1 env2 t1
-  | TTPair t1 t2
-  | TTUnion t1 t2
-  | TTTable t1 t2
-    ->
-      impl_type_sem_incr cbor_t env1 env2 t1;
-      impl_type_sem_incr cbor_t env1 env2 t2
-  | _ -> ()
-
-[@sem_attr]
-noeq
-type rel_env
-  (#bound: name_env)
-  (s_env: target_type_env bound)
-= {
-  r_type: target_impl_env bound;
-  r_rel: (n: typ_name bound) -> rel (r_type n) (s_env.te_type n);
-}
-
-let rec rel_type_sem
-  (#bound: name_env)
-  (cbor_t: Type0)
-  (vmatch: perm -> cbor_t -> Cbor.cbor -> slprop)
-  (#s_env: target_type_env bound)
-  (env: rel_env s_env)
-  (t: target_type { target_type_bounded bound t })
-: Tot (rel (impl_type_sem cbor_t env.r_type t) (target_type_sem s_env.te_type t) )
-  (decreases t)
-= match t returns rel (impl_type_sem cbor_t env.r_type t) (target_type_sem s_env.te_type t) with
-  | TTDef s -> env.r_rel s
-  | TTElem elt -> rel_elem_type_sem vmatch elt
-  | TTOption t -> rel_option (rel_type_sem cbor_t vmatch env t)
-  | TTPair t1 t2 -> rel_pair (rel_type_sem cbor_t vmatch env t1) (rel_type_sem cbor_t vmatch env t2)
-  | TTUnion t1 t2 -> rel_either (rel_type_sem cbor_t vmatch env t1) (rel_type_sem cbor_t vmatch env t2)
-  | TTArray t -> rel_slice_of_list (rel_type_sem cbor_t vmatch env t) false
-  | TTTable t1 t2 -> rel_slice_of_table (target_type_eq s_env t1) (rel_type_sem cbor_t vmatch env t1) (rel_type_sem cbor_t vmatch env t2)
+  | TTElem elt -> { sem_impl_type = impl_elem_type_sem cbor_t elt; sem_rel = rel_elem_type_sem vmatch elt }
+  | TTOption t ->
+    let it = impl_type_sem vmatch env t in {
+      sem_impl_type = option it.sem_impl_type;
+      sem_rel = rel_option it.sem_rel
+    }
+  | TTPair t1 t2 ->
+    let it1 = impl_type_sem vmatch env t1 in
+    let it2 = impl_type_sem vmatch env t2 in {
+      sem_impl_type = (it1.sem_impl_type & it2.sem_impl_type);
+      sem_rel = rel_pair it1.sem_rel it2.sem_rel
+    }
+  | TTUnion t1 t2 ->
+    let it1 = impl_type_sem vmatch env t1 in
+    let it2 = impl_type_sem vmatch env t2 in {
+      sem_impl_type = (it1.sem_impl_type `either` it2.sem_impl_type);
+      sem_rel = rel_either it1.sem_rel it2.sem_rel
+    }
+  | TTArray t ->
+    let it = impl_type_sem vmatch env t in {
+      sem_impl_type = slice it.sem_impl_type; // HERE we will plug support for iterable CBOR arrays whose elements will be parsed wrt. it.sem_rel
+      sem_rel = rel_slice_of_list it.sem_rel false;
+    }
+  | TTTable t1 t2 ->
+    let it1 = impl_type_sem vmatch env t1 in
+    let it2 = impl_type_sem vmatch env t2 in {
+      sem_impl_type = slice (it1.sem_impl_type & it2.sem_impl_type); // HERE we will plug support for iterable CBOR maps whose elements will be parsed wrt. it1.sem_rel, it2.sem_rel
+      sem_rel = rel_slice_of_table (target_type_eq s_env t1) it1.sem_rel it2.sem_rel
+    }
 
 let rel_env_included
   (#bound1: name_env)
@@ -144,10 +111,9 @@ let rel_env_included
   (r2: rel_env s_env2)
 : Tot prop
 = target_spec_env_included s_env1.te_type s_env2.te_type /\
-  target_impl_env_included r1.r_type r2.r_type /\
-  (forall (n: typ_name bound1) . r1.r_rel n == coerce_eq () (r2.r_rel n))
+  (forall (n: typ_name bound1) . r1 n == coerce_eq () (r2 n))
 
-let rec rel_type_sem_incr
+let rec impl_type_sem_incr
   (#bound1: name_env)
   (cbor_t: Type0)
   (vmatch: perm -> cbor_t -> Cbor.cbor -> slprop)
@@ -161,20 +127,20 @@ let rec rel_type_sem_incr
   (requires rel_env_included env1 env2 /\
     target_type_bounded bound1 t
   )
-  (ensures rel_type_sem cbor_t vmatch env1 t == coerce_eq () (rel_type_sem cbor_t vmatch env2 t)) // FIXME: WHY WHY WHY do we have this coerce_eq?
+  (ensures impl_type_sem vmatch env1 t == coerce_eq () (impl_type_sem vmatch env2 t)) // FIXME: WHY WHY WHY do we have this coerce_eq?
   (decreases t)
   [SMTPatOr [
-    [SMTPat (rel_env_included env1 env2); SMTPat (rel_type_sem cbor_t vmatch env1 t);];
-    [SMTPat (rel_env_included env1 env2); SMTPat (rel_type_sem cbor_t vmatch env2 t);];
+    [SMTPat (rel_env_included env1 env2); SMTPat (impl_type_sem vmatch env1 t);];
+    [SMTPat (rel_env_included env1 env2); SMTPat (impl_type_sem vmatch env2 t);];
   ]]
 = match t with
   | TTOption t1
   | TTArray t1
-    -> rel_type_sem_incr cbor_t vmatch env1 env2 t1
+    -> impl_type_sem_incr cbor_t vmatch env1 env2 t1
   | TTPair t1 t2
   | TTUnion t1 t2
   | TTTable t1 t2 ->
     eq_test_unique (target_type_eq s_env1 t1) (coerce_eq () (target_type_eq s_env2 t1));
-    rel_type_sem_incr cbor_t vmatch env1 env2 t1;
-    rel_type_sem_incr cbor_t vmatch env1 env2 t2
+    impl_type_sem_incr cbor_t vmatch env1 env2 t1;
+    impl_type_sem_incr cbor_t vmatch env1 env2 t2
   | _ -> ()
